redo proof of HReduce via approximation

dist/Kuiper_ZeroKernel.cu
@@ -15,6 +15,6 @@ void Kuiper_ZeroKernel_test(void)
     KPR_SHMEM_FITS(0U);
     MUST(cudaFuncSetAttribute
          (__hoisted_0, cudaFuncAttributeMaxDynamicSharedMemorySize, 0U));
-    KPR_KCALL(__hoisted_0, 0U, 0U, 0U);
+    KPR_KCALL(__hoisted_0, 1U, 0U, 0U);
     MUST(cudaDeviceSynchronize());
 }
