src/lib/kuiper/Kuiper.Approximates.fsti
@@ -3,9 +3,19 @@ module Kuiper.Approximates
 open Kuiper
 open FStar.Real
 open Kuiper.Scalars
+open Kuiper.Seq.Common
 
 class real_like (a:Type) {| scalar a |} = {
+  to_real : a -> real;
+
   approximates : a -> real -> prop;
+
+  to_real_ok :
+    x:a ->
+    Lemma (ensures x `approximates` to_real x)
+          [SMTPat (x `approximates` to_real x)];
+
+  (* We assume these two values exist and approximate correctly *)
 
   a0 : squash (approximates zero 0.0R);
   a1 : squash (approximates one 1.0R);
@@ -14,11 +24,13 @@ class real_like (a:Type) {| scalar a |} = {
           Lemma (requires approximates x r /\ approximates y s)
                 (ensures approximates (x `add` y) (r +. s))
                 [SMTPat (approximates x r); SMTPat (approximates y s)];
+                // ^ Does not kick in
 
   a_mul : x:a -> y:a -> r:real -> s:real ->
           Lemma (requires approximates x r /\ approximates y s)
                 (ensures approximates (x `mul` y) (r *. s))
                 [SMTPat (approximates x r); SMTPat (approximates y s)];
+                // ^ Does not kick in
 }
 
 (* We assume these types approximate reals *)
@@ -33,3 +45,27 @@ instance val real_like_u8 : real_like u8
 instance val real_like_u16 : real_like u16
 instance val real_like_u32 : real_like u32
 instance val real_like_u64 : real_like u64
+
+let seq_approximates (#a:Type) {| scalar a, real_like a |}
+  (s : seq a) (r : seq Real.real) : prop
+  = Seq.length s == Seq.length r /\
+    (forall i. i < len s ==> (s @! i) `approximates` (r @! i))
+
+let to_real_seq (#a:Type) {| scalar a, real_like a |}
+  (s : seq a) : GTot (seq Real.real)
+  = Seq.init_ghost (Seq.length s) (fun i -> to_real (s @! i))
+
+let real_seq_sum (r : seq Real.real) : Real.real
+  = seq_fold_left (+.) 0.0R r
+
+let real_seq_sum_append
+  (r1 r2 : seq Real.real)
+  : Lemma (real_seq_sum (r1 `Seq.append` r2) == real_seq_sum r1 +. real_seq_sum r2)
+  = admit()
+
+let seq_approximates_append (#a:Type) {| scalar a, real_like a |}
+  (s1 s2 : a) (r1 r2 : seq Real.real)
+  : Lemma (requires s1 `approximates` real_seq_sum r1 /\ s2 `approximates` real_seq_sum r2)
+          (ensures (s1 `add` s2) `approximates` real_seq_sum (r1 `Seq.append` r2))
+  = a_add s1 s2 (real_seq_sum r1) (real_seq_sum r2);
+    real_seq_sum_append r1 r2
